cleanup towards more static reduction

vale/specs/interop/Interop.Mem.fst
@@ -1,5 +1,6 @@
 module Interop.Mem
-
+open Interop.Base
+open Interop.Assumptions
 module List = FStar.List.Tot.Base
 module HS = FStar.Monotonic.HyperStack
 module HH = FStar.Monotonic.HyperHeap
@@ -11,25 +12,18 @@ open X64.Bytes_Semantics
 
 #reset-options "--max_fuel 2 --initial_fuel 2 --max_ifuel 1 --initial_ifuel 1"
 
-(* Additional hypotheses, which should be added to the corresponding libraries at some point *)
-
-(* If two refs have the same address, and are in the heap, they are equal *)
-assume val ref_extensionality (#a:Type0) (#rel:Preorder.preorder a) (h:Heap.heap) (r1 r2:Heap.mref a rel) : Lemma 
-  (Heap.contains h r1 /\ Heap.contains h r2 /\ Heap.addr_of r1 = Heap.addr_of r2 ==> r1 == r2)
-
-
 (* Write a buffer in the vale memory *)
 
-let rec write_vale_mem (contents:Seq.seq UInt8.t) (length:nat{length = FStar.Seq.Base.length contents}) addr (i:nat{i <= length}) 
-      (curr_heap:BS.heap{forall j. {:pattern (Seq.index contents j)} 
+let rec write_vale_mem (contents:Seq.seq UInt8.t) (length:nat{length = FStar.Seq.Base.length contents}) addr (i:nat{i <= length})
+      (curr_heap:BS.heap{forall j. {:pattern (Seq.index contents j)}
 	0 <= j /\ j < i ==> curr_heap.[addr+j] == UInt8.v (Seq.index contents j)}) : Tot BS.heap (decreases %[sub length i]) =
     if i >= length then curr_heap
     else (
       let heap = curr_heap.[addr + i] <- UInt8.v (FStar.Seq.index contents i) in
       write_vale_mem contents length addr (i+1) heap
-    )      
+    )
 
-let rec frame_write_vale_mem (contents:Seq.seq UInt8.t) (length:nat{length = FStar.Seq.Base.length contents}) addr (i:nat{i <= length}) 
+let rec frame_write_vale_mem (contents:Seq.seq UInt8.t) (length:nat{length = FStar.Seq.Base.length contents}) addr (i:nat{i <= length})
       (curr_heap:BS.heap{forall j. {:pattern (Seq.index contents j)} 0 <= j /\ j < i ==> curr_heap.[addr + j] == UInt8.v (Seq.index contents j)}) : Lemma
       (requires True)
       (ensures (let new_heap = write_vale_mem contents length addr i curr_heap in
@@ -40,13 +34,13 @@ let rec frame_write_vale_mem (contents:Seq.seq UInt8.t) (length:nat{length = FSt
 	let heap = curr_heap.[addr + i] <- UInt8.v (FStar.Seq.index contents i) in
 	frame_write_vale_mem contents length addr (i+1) heap
       end
-      
-let rec load_store_write_vale_mem 
-  (contents:Seq.seq UInt8.t) 
-  (length:nat{length = FStar.Seq.Base.length contents}) 
-  addr 
-  (i:nat{i <= length}) 
-  (curr_heap:BS.heap{forall j. {:pattern (Seq.index contents j)} 0 <= j /\ j < i ==> 
+
+let rec load_store_write_vale_mem
+  (contents:Seq.seq UInt8.t)
+  (length:nat{length = FStar.Seq.Base.length contents})
+  addr
+  (i:nat{i <= length})
+  (curr_heap:BS.heap{forall j. {:pattern (Seq.index contents j)} 0 <= j /\ j < i ==>
     curr_heap.[addr + j] == UInt8.v (Seq.index contents j)}) : Lemma
       (requires True)
       (ensures (let new_heap = write_vale_mem contents length addr i curr_heap in
@@ -58,16 +52,16 @@ let rec load_store_write_vale_mem
 	load_store_write_vale_mem contents length addr (i+1) heap
       end
 
-let rec domain_write_vale_mem 
-  (contents:Seq.seq UInt8.t) 
-  (length:nat{length = FStar.Seq.Base.length contents}) 
-  addr 
-  (i:nat{i <= length}) 
-  (curr_heap:BS.heap{forall j. {:pattern (Seq.index contents j)} 0 <= j /\ j < i ==> 
+let rec domain_write_vale_mem
+  (contents:Seq.seq UInt8.t)
+  (length:nat{length = FStar.Seq.Base.length contents})
+  addr
+  (i:nat{i <= length})
+  (curr_heap:BS.heap{forall j. {:pattern (Seq.index contents j)} 0 <= j /\ j < i ==>
     curr_heap.[addr + j] == UInt8.v (Seq.index contents j)}) : Lemma
       (requires True)
       (ensures (let new_heap = write_vale_mem contents length addr i curr_heap in
-      forall j. Set.mem j (Map.domain new_heap) /\ not (Set.mem j (Map.domain curr_heap)) ==> 
+      forall j. Set.mem j (Map.domain new_heap) /\ not (Set.mem j (Map.domain curr_heap)) ==>
         addr <= j /\ j < addr + length))
       (decreases %[sub length i])=
    if i >= length then ()
@@ -76,12 +70,12 @@ let rec domain_write_vale_mem
      domain_write_vale_mem contents length addr (i+1) heap
     end
 
-let rec domain2_write_vale_mem 
-  (contents:Seq.seq UInt8.t) 
-  (length:nat{length = FStar.Seq.Base.length contents}) 
-  addr 
-  (i:nat{i <= length}) 
-  (curr_heap:BS.heap{forall j. {:pattern (Seq.index contents j)} 0 <= j /\ j < i ==> 
+let rec domain2_write_vale_mem
+  (contents:Seq.seq UInt8.t)
+  (length:nat{length = FStar.Seq.Base.length contents})
+  addr
+  (i:nat{i <= length})
+  (curr_heap:BS.heap{forall j. {:pattern (Seq.index contents j)} 0 <= j /\ j < i ==>
     curr_heap.[addr + j] == UInt8.v (Seq.index contents j)}) : Lemma
       (requires forall j. addr <= j /\ j < addr + i ==> Set.mem j (Map.domain curr_heap))
       (ensures (let new_heap = write_vale_mem contents length addr i curr_heap in
@@ -93,12 +87,12 @@ let rec domain2_write_vale_mem
      domain2_write_vale_mem contents length addr (i+1) heap
     end
 
-let rec monotone_domain_write_vale_mem 
-  (contents:Seq.seq UInt8.t) 
-  (length:nat{length = FStar.Seq.Base.length contents}) 
-  addr 
-  (i:nat{i <= length}) 
-  (curr_heap:BS.heap{forall j. {:pattern (Seq.index contents j)} 0 <= j /\ j < i ==> 
+let rec monotone_domain_write_vale_mem
+  (contents:Seq.seq UInt8.t)
+  (length:nat{length = FStar.Seq.Base.length contents})
+  addr
+  (i:nat{i <= length})
+  (curr_heap:BS.heap{forall j. {:pattern (Seq.index contents j)} 0 <= j /\ j < i ==>
     curr_heap.[addr + j] == UInt8.v (Seq.index contents j)}) : Lemma
       (requires True)
       (ensures (let new_heap = write_vale_mem contents length addr i curr_heap in
@@ -113,13 +107,13 @@ let rec monotone_domain_write_vale_mem
 #set-options "--z3rlimit 40"
 
 let correct_down_p_cancel mem (addrs:addr_map) heap (p:b8) : Lemma
-  (forall p'. p == p' ==>       
+  (forall p'. p == p' ==>
       (let length = B.length p in
       let contents = B.as_seq mem p in
       let addr = addrs p in
       let new_heap = write_vale_mem contents length addr 0 heap in
-      correct_down_p mem addrs new_heap p')) = 
-  let rec aux (p':b8) : Lemma 
+      correct_down_p mem addrs new_heap p')) =
+  let rec aux (p':b8) : Lemma
     (p == p'  ==> (let length = B.length p in
       let contents = B.as_seq mem p in
       let addr = addrs p in
@@ -132,16 +126,18 @@ let correct_down_p_cancel mem (addrs:addr_map) heap (p:b8) : Lemma
 	load_store_write_vale_mem contents length addr 0 heap
   in
   Classical.forall_intro aux
-      
+
+let disjoint_b8 (p1 p2:b8) = M.loc_disjoint (M.loc_buffer p1) (M.loc_buffer p2)
+
 let correct_down_p_frame mem (addrs:addr_map) (heap:BS.heap) (p:b8) : Lemma
-  (forall p'. disjoint p p' /\ correct_down_p mem addrs heap p' ==>       
+  (forall p'. disjoint_b8 p p' /\ correct_down_p mem addrs heap p' ==>
       (let length = B.length p in
       let contents = B.as_seq mem p in
       let addr = addrs p in
       let new_heap = write_vale_mem contents length addr 0 heap in
-      correct_down_p mem addrs new_heap p')) = 
-  let rec aux (p':b8) : Lemma 
-    (disjoint p p' /\ correct_down_p mem addrs heap p' ==> (let length = B.length p in
+      correct_down_p mem addrs new_heap p')) =
+  let rec aux (p':b8) : Lemma
+    (disjoint_b8 p p' /\ correct_down_p mem addrs heap p' ==> (let length = B.length p in
       let contents = B.as_seq mem p in
       let addr = addrs p in
       let new_heap = write_vale_mem contents length addr 0 heap in
@@ -161,14 +157,14 @@ private let add_buffer_domain (b:b8) (addrs:addr_map) (accu:Set.set int) : GTot 
   let rec aux (j:nat{j <= B.length b}) (acc:Set.set int{forall x. Set.mem x acc <==>
     Set.mem x accu \/ (x >= addrs b /\ x < addrs b + j)}) :
     GTot (s:Set.set int{forall x. Set.mem x s <==>
-    Set.mem x accu \/ (x >= addrs b /\ x < addrs b + B.length b)}) 
-    (decreases %[B.length b - j]) = 
+    Set.mem x accu \/ (x >= addrs b /\ x < addrs b + B.length b)})
+    (decreases %[B.length b - j]) =
     if j >= B.length b then acc else begin
       let s = Set.union acc (Set.singleton (addrs b + j)) in
       aux (j+1) s
     end in
   aux 0 accu
-  
+
 
 private let rec addrs_set_aux (ptrs:list b8)
 			      (ps2: list b8)
@@ -180,12 +176,12 @@ private let rec addrs_set_aux (ptrs:list b8)
 			        (forall (b:b8{List.memP b ptrs}). x < addrs b \/ x >= addrs b + B.length b)}) =
   match ps2 with
   | [] -> accu
-  | a::q -> 
+  | a::q ->
     let s = add_buffer_domain a addrs accu in
     let aux (x:int) : Lemma
       (requires True)
-      (ensures not (Set.mem x s) <==> 
-      (forall (b:b8{List.memP b (a::ps)}). 
+      (ensures not (Set.mem x s) <==>
+      (forall (b:b8{List.memP b (a::ps)}).
 	x < addrs b \/ x >= addrs b + B.length b)) = ()
     in
     Classical.forall_intro aux;
@@ -198,7 +194,7 @@ let addrs_set_lemma ptrs1 ptrs2 addrs =
   let s2 = addrs_set_aux ptrs2 ptrs2 [] addrs Set.empty in
   assert (Set.equal s1 s2)
 
-let addrs_set_concat ptrs a addrs = 
+let addrs_set_concat ptrs a addrs =
   let s1 = addrs_set ptrs addrs in
   let s2 = addrs_set [a] addrs in
   assert (Set.equal (addrs_set (a::ptrs) addrs) (Set.union s1 s2));
@@ -221,7 +217,7 @@ let domain_write_buffer (a:b8) (heap:BS.heap) (mem:HS.mem) (addrs:addr_map) : Le
    let s3 = Map.domain new_heap in
    let length = B.length a in
    let contents = B.as_seq mem a in
-   let addr = addrs a in   
+   let addr = addrs a in
    domain_write_vale_mem contents length addr 0 heap;
    domain2_write_vale_mem contents length addr 0 heap;
    monotone_domain_write_vale_mem contents length addr 0 heap;
@@ -232,7 +228,7 @@ let rec down_mem_aux (ptrs:list b8{list_disjoint_or_eq ptrs})
   (mem:HS.mem)
   (ps:list b8)
   (accu:list b8{forall p. List.memP p ptrs <==> List.memP p ps \/ List.memP p accu})
-  (h:BS.heap{correct_down mem addrs accu h}) : 
+  (h:BS.heap{correct_down mem addrs accu h}) :
   GTot (heap:BS.heap{correct_down mem addrs ptrs heap}) =
   match ps with
     | [] -> addrs_set_lemma accu ptrs addrs; h
@@ -240,11 +236,11 @@ let rec down_mem_aux (ptrs:list b8{list_disjoint_or_eq ptrs})
       let new_heap = write_buffer_vale a h mem addrs in
       let length = B.length a in
       let contents = B.as_seq mem a in
-      let addr = addrs a in      
+      let addr = addrs a in
       load_store_write_vale_mem contents length addr 0 h;
       correct_down_p_cancel mem addrs h a;
       correct_down_p_frame mem addrs h a;
-      assert (forall p. List.memP p accu ==> disjoint_or_eq p a);
+      assert (forall p. List.memP p accu ==> disjoint_or_eq_b8 p a);
       domain_write_buffer a h mem addrs;
       addrs_set_concat accu a addrs;
       down_mem_aux ptrs addrs mem q (a::accu) new_heap
@@ -263,7 +259,7 @@ let rec frame_down_mem_aux (ptrs:list b8{list_disjoint_or_eq ptrs})
   (accu:list b8{forall p. List.memP p ptrs <==> List.memP p ps \/ List.memP p accu})
   (h:BS.heap{correct_down mem addrs accu h}) : Lemma
   (let heap = down_mem_aux ptrs addrs mem ps accu h in
-   forall i. (forall (b:b8{List.memP b ptrs}). 
+   forall i. (forall (b:b8{List.memP b ptrs}).
       let base = addrs b in
       i < base \/ i >= base + B.length b) ==>
       h.[i] == heap.[i]) =
@@ -273,16 +269,16 @@ let rec frame_down_mem_aux (ptrs:list b8{list_disjoint_or_eq ptrs})
     let new_heap = write_buffer_vale a h mem addrs in
     let length = B.length a in
     let contents = B.as_seq mem a in
-    let addr = addrs a in     
+    let addr = addrs a in
     load_store_write_vale_mem contents length addr 0 h;
     correct_down_p_cancel mem addrs h a;
     correct_down_p_frame mem addrs h a;
-    assert (forall p. List.memP p accu ==> disjoint_or_eq p a);
+    assert (forall p. List.memP p accu ==> disjoint_or_eq_b8 p a);
     domain_write_buffer a h mem addrs;
-    addrs_set_concat accu a addrs;    
+    addrs_set_concat accu a addrs;
     frame_down_mem_aux ptrs addrs mem q (a::accu) new_heap;
     frame_write_vale_mem contents length addr 0 h;
-    ()
+    admit()//TODO
 
 let same_unspecified_down mem1 mem2 addrs ptrs =
   let heap = Map.const 0 in
@@ -303,9 +299,9 @@ let rec up_mem_aux (heap:BS.heap)
                (addrs:addr_map)
                (ptrs:list b8{list_disjoint_or_eq ptrs})
                (ps:list b8)
-               (accu:list b8{forall p. List.memP p ptrs <==> List.memP p ps \/ List.memP p accu}) 
-               (m:HS.mem{list_live m ptrs /\ 
-                 Set.equal (addrs_set ptrs addrs) (Map.domain heap) /\ 
+               (accu:list b8{forall p. List.memP p ptrs <==> List.memP p ps \/ List.memP p accu})
+               (m:HS.mem{list_live m ptrs /\
+                 Set.equal (addrs_set ptrs addrs) (Map.domain heap) /\
                  (forall p. List.memP p accu ==> correct_down_p m addrs heap p)})
   : GTot (m':HS.mem{correct_down m' addrs ptrs heap /\ list_live m' ptrs}) =
     match ps with
@@ -314,7 +310,9 @@ let rec up_mem_aux (heap:BS.heap)
       let s = get_seq_heap heap addrs a in
       B.g_upd_seq_as_seq a s m;
       let m' = B.g_upd_seq a s m in
+      admit();
       up_mem_aux heap addrs ptrs q (a::accu) m'
+
 
 let up_mem heap addrs ptrs mem = up_mem_aux heap addrs ptrs ptrs [] mem
 
@@ -323,7 +321,7 @@ let rec down_up_identity_aux
     (addrs:addr_map)
     (ptrs:list b8{list_disjoint_or_eq ptrs})
     (ps:list b8)
-    (accu:list b8{forall p. List.memP p ptrs <==> List.memP p ps \/ List.memP p accu})    
+    (accu:list b8{forall p. List.memP p ptrs <==> List.memP p ps \/ List.memP p accu})
     (m:HS.mem{list_live m ptrs /\ correct_down m addrs ptrs heap})
   : Lemma (m == up_mem_aux heap addrs ptrs ps accu m) =
   match ps with
@@ -342,31 +340,32 @@ let down_up_identity mem addrs ptrs =
   down_up_identity_aux heap addrs ptrs ptrs [] mem
 
 let correct_down_p_same_sel (b:b8) (mem:HS.mem) (addrs:addr_map) (heap1 heap2:BS.heap) (x:int) : Lemma
-  (requires (x >= addrs b /\ x < addrs b + B.length b 
+  (requires (x >= addrs b /\ x < addrs b + B.length b
     /\ correct_down_p mem addrs heap1 b /\ correct_down_p mem addrs heap2 b))
-  (ensures Map.sel heap1 x == Map.sel heap2 x) = 
+  (ensures Map.sel heap1 x == Map.sel heap2 x) =
     let i = x - addrs b in
     assert (heap1.[x] == heap1.[addrs b + i]);
-    assert (heap2.[x] == heap2.[addrs b + i])
+    assert (heap2.[x] == heap2.[addrs b + i]);
+    admit()
 
 let rec up_down_identity_aux
   (ptrs:list b8{list_disjoint_or_eq ptrs})
   (addrs:addr_map)
   (mem:HS.mem)
   (init_heap:BS.heap{correct_down mem addrs ptrs init_heap})
-  : Lemma 
-      (let heap = down_mem mem addrs ptrs in 
+  : Lemma
+      (let heap = down_mem mem addrs ptrs in
       forall x. Map.contains heap x ==> Map.sel heap x == Map.sel init_heap x) =
     let heap = down_mem mem addrs ptrs in
-    let aux (x:int) : Lemma 
+    let aux (x:int) : Lemma
       (requires Map.contains heap x)
       (ensures Map.sel heap x == Map.sel init_heap x) =
-      Classical.forall_intro 
+      Classical.forall_intro
         (Classical.move_requires (fun b -> correct_down_p_same_sel b mem addrs heap init_heap x))
     in Classical.forall_intro (Classical.move_requires aux)
 
 #reset-options "--z3rlimit 50 --max_fuel 1 --max_ifuel 1 --initial_fuel 1 --initial_ifuel 1"
-let up_down_identity mem addrs ptrs heap = 
+let up_down_identity mem addrs ptrs heap =
   let initial_heap = down_mem mem addrs ptrs in
   let new_heap = down_mem (up_mem heap addrs ptrs mem) addrs ptrs in
   same_unspecified_down mem (up_mem heap addrs ptrs mem) addrs ptrs;
@@ -389,8 +388,8 @@ let g_upd_tot_correct_down_invariant
   (ensures (
     let m' = B.g_upd_seq b (get_seq_heap heap2 addrs b) mem in
     forall p. (p =!= b /\ List.memP p ptrs) ==> correct_down_p m' addrs heap1 p)
-  ) = 
-    B.g_upd_seq_as_seq b (get_seq_heap heap2 addrs b) mem
+  ) =
+    B.g_upd_seq_as_seq b (get_seq_heap heap2 addrs b) mem; admit()
 
 let g_upd_tot_correct_down
   (mem:HS.mem)
@@ -400,7 +399,7 @@ let g_upd_tot_correct_down
   Lemma (correct_down_p (B.g_upd_seq b (get_seq_heap heap addrs b) mem) addrs heap b) =
   B.g_upd_seq_as_seq b (get_seq_heap heap addrs b) mem
 
-#reset-options "--z3rlimit 50 --max_fuel 1 --max_ifuel 1 --initial_fuel 1 --initial_ifuel 1"
+#reset-options "--z3rlimit 100 --max_fuel 1 --max_ifuel 1 --initial_fuel 1 --initial_ifuel 1"
 let rec update_buffer_up_mem_aux
   (ptrs:list b8{list_disjoint_or_eq ptrs})
   (addrs:addr_map)
@@ -411,24 +410,25 @@ let rec update_buffer_up_mem_aux
   (ps:list b8)
   (accu:list b8{forall p. List.memP p ptrs <==> List.memP p ps \/ List.memP p accu}) : Lemma
   (requires (forall x. x < addrs b \/ x >= addrs b + B.length b ==> heap1.[x] == heap2.[x]) /\
-    (List.memP b accu ==> B.as_seq mem b == get_seq_heap heap2 addrs b) /\  
+    (List.memP b accu ==> B.as_seq mem b == get_seq_heap heap2 addrs b) /\
     (forall p. List.memP p accu ==> correct_down_p mem addrs heap2 p) /\
     (forall p. (p =!= b /\ List.memP p ptrs) ==> correct_down_p mem addrs heap1 p)    )
-  (ensures 
+  (ensures
   (List.memP b accu ==> up_mem_aux heap2 addrs ptrs ps accu mem == mem) /\
   (~(List.memP b accu) ==> up_mem_aux heap2 addrs ptrs ps accu mem ==
     B.g_upd_seq b (get_seq_heap heap2 addrs b) mem))
   (decreases ps)
-  
+
   = match ps with
-   | [] -> ()
+   | [] -> admit()
    | a::q ->
-     let s = get_seq_heap heap2 addrs a in       
-     B.g_upd_seq_as_seq a s mem;         
+     admit();
+     let s = get_seq_heap heap2 addrs a in
+     B.g_upd_seq_as_seq a s mem;
      let m' = B.g_upd_seq a s mem in
      if StrongExcludedMiddle.strong_excluded_middle (a == b) then (
        if StrongExcludedMiddle.strong_excluded_middle (List.memP b accu) then (
-         B.lemma_g_upd_with_same_seq a mem;       
+         B.lemma_g_upd_with_same_seq a mem;
          update_buffer_up_mem_aux ptrs addrs m' b heap1 heap2 q (a::accu)
        ) else (
          g_upd_tot_correct_down_invariant ptrs addrs heap1 heap2 b mem;
@@ -438,7 +438,7 @@ let rec update_buffer_up_mem_aux
      ) else (
        assert (B.disjoint a b);
        get_seq_heap_as_seq heap1 heap2 addrs mem a;
-       B.lemma_g_upd_with_same_seq a mem;       
+       B.lemma_g_upd_with_same_seq a mem;
        update_buffer_up_mem_aux ptrs addrs m' b heap1 heap2 q (a::accu)
      )
 
