vale/specs/interop/Interop.Mem.fsti
@@ -1,5 +1,5 @@
 module Interop.Mem
-
+open Interop.Base
 module List = FStar.List.Tot.Base
 module HS = FStar.Monotonic.HyperStack
 module HH = FStar.Monotonic.HyperHeap
@@ -11,51 +11,22 @@ module BS = X64.Bytes_Semantics_s
 let op_String_Access = Map.sel
 let op_String_Assignment = Map.upd
 
-inline_for_extraction
-let b8 = B.buffer UInt8.t
-
 let sub l i = l - i
 
-let rec loc_locs_disjoint_rec (l:b8) (ls:list b8) : Type0 =
-  match ls with
-  | [] -> True
-  | h::t -> M.loc_disjoint (M.loc_buffer l) (M.loc_buffer h) /\ loc_locs_disjoint_rec l t
+[@__reduce__]
+let disjoint_or_eq_b8 (ptr1 ptr2:b8) = M.loc_disjoint (M.loc_buffer ptr1) (M.loc_buffer ptr2) \/ ptr1 == ptr2
 
-let rec locs_disjoint_rec (ls:list b8) : Type0 =
-  match ls with
-  | [] -> True
-  | h::t -> loc_locs_disjoint_rec h t /\ locs_disjoint_rec t
+[@__reduce__]
+let disjoint_or_eq_b8_l (ptrs:list b8)
+ : prop
+ = BigOps.pairwise_and disjoint_or_eq_b8 ptrs
 
-unfold
-let bufs_disjoint (ls:list b8) : Type0 =
-  norm [iota; zeta; delta; delta_only [`%loc_locs_disjoint_rec;
-                                       `%locs_disjoint_rec]] (locs_disjoint_rec ls)
+let list_disjoint_or_eq (ptrs:list b8) =
+  forall (p1 p2:b8). List.memP p1 ptrs /\ List.memP p2 ptrs ==> disjoint_or_eq_b8 p1 p2
 
 unfold
-let buf_disjoint_from (b:b8) (ls:list b8) : Type0 =
-  norm [iota; zeta; delta; delta_only [`%loc_locs_disjoint_rec;
-                                       `%locs_disjoint_rec]] (loc_locs_disjoint_rec b ls)
-
-unfold
-let disjoint (#a:Type0) (ptr1 ptr2:B.buffer a) = M.loc_disjoint (M.loc_buffer ptr1) (M.loc_buffer ptr2)
-
-unfold
-let disjoint_or_eq ptr1 ptr2 = disjoint ptr1 ptr2 \/ ptr1 == ptr2
-
-let list_disjoint_or_eq (#a:Type0) (ptrs:list (B.buffer a)) =
-  forall p1 p2. List.memP p1 ptrs /\ List.memP p2 ptrs ==> disjoint_or_eq p1 p2
-
-let disjoint_addr addr1 length1 addr2 length2 =
-  (* The first buffer is completely before the second, or the opposite *)
-  addr1 + length1 < addr2 || addr2 + length2 < addr1
-
-type addr_map = (m:(b8 -> MS.nat64){
-  (forall (buf1 buf2:b8).{:pattern (m buf1); (m buf2)} disjoint buf1 buf2 ==> 
-    disjoint_addr (m buf1) (B.length buf1) (m buf2) (B.length buf2)) /\
-  (forall (b:b8).{:pattern (m b)} m b + B.length b < MS.pow2_64)})
-
-unfold
-let list_live (#a:Type0) mem (ptrs:list (B.buffer a)) = forall p . List.memP p ptrs ==> B.live mem p
+let list_live (#a:Type0) mem (ptrs:list (B.buffer a)) =
+  forall p . List.memP p ptrs ==> B.live mem p
 
 let correct_down_p (mem:HS.mem) (addrs:addr_map) (heap:BS.heap) (p:b8) =
   let length = B.length p in
@@ -63,21 +34,24 @@ let correct_down_p (mem:HS.mem) (addrs:addr_map) (heap:BS.heap) (p:b8) =
   let addr = addrs p in
   (forall i.  0 <= i /\ i < length ==> heap.[addr + i] == UInt8.v (FStar.Seq.index contents i))
 
-val addrs_set: (ptrs:list b8) -> (addrs:addr_map) -> GTot (s:Set.set int{
-  forall x.{:pattern (Set.mem x s)} not (Set.mem x s) <==> 
-    (forall (b:b8{List.memP b ptrs}).{:pattern (addrs b)} x < addrs b \/ x >= addrs b + B.length b)})
+val addrs_set (ptrs:list b8) (addrs:addr_map)
+  : GTot (s:Set.set int{
+                 forall x.{:pattern (Set.mem x s)}
+                   not (Set.mem x s) <==> 
+                   (forall (b:b8{List.memP b ptrs}).{:pattern (addrs b)}
+                     x < addrs b \/ x >= addrs b + B.length b)})
     
-val addrs_set_lemma: (ptrs1:list b8) -> (ptrs2:list b8) ->
-  (addrs:addr_map) -> Lemma
-  (requires forall b. List.memP b ptrs1 <==> List.memP b ptrs2)
-  (ensures addrs_set ptrs1 addrs == addrs_set ptrs2 addrs)
+val addrs_set_lemma (ptrs1:list b8) (ptrs2:list b8) (addrs:addr_map)
+  : Lemma
+    (requires forall b. List.memP b ptrs1 <==> List.memP b ptrs2)
+    (ensures addrs_set ptrs1 addrs == addrs_set ptrs2 addrs)
 
-val addrs_set_concat: (ptrs:list b8) -> (a:b8) ->
-  (addrs:addr_map) -> Lemma
-  (addrs_set (a::ptrs) addrs == Set.union (addrs_set ptrs addrs) (addrs_set [a] addrs))
+val addrs_set_concat (ptrs:list b8) (a:b8) (addrs:addr_map)
+  : Lemma
+    (addrs_set (a::ptrs) addrs == Set.union (addrs_set ptrs addrs) (addrs_set [a] addrs))
   
-val addrs_set_mem: (ptrs:list b8) -> (a:b8) ->
-  (addrs:addr_map) -> (i:int) -> Lemma
+val addrs_set_mem (ptrs:list b8) (a:b8) (addrs:addr_map) (i:int)
+  : Lemma
   (requires List.memP a ptrs /\ i >= addrs a /\ i < addrs a + B.length a)
   (ensures Set.mem i (addrs_set ptrs addrs))
   
@@ -86,7 +60,8 @@ let correct_down mem (addrs:addr_map) (ptrs: list b8) heap =
   (forall p. List.memP p ptrs ==> correct_down_p mem addrs heap p)
 
 (* Takes a Low* Hyperstack and a list of buffers and create a vale memory + keep track of the vale addresses *)
-val down_mem: (mem:HS.mem) -> (addrs: addr_map) -> (ptrs:list b8{list_disjoint_or_eq ptrs}) -> GTot (heap :BS.heap {correct_down mem addrs ptrs heap})
+val down_mem (mem:HS.mem) (addrs: addr_map) (ptrs:list b8{list_disjoint_or_eq ptrs})
+  : GTot (heap :BS.heap {correct_down mem addrs ptrs heap})
 
 val same_unspecified_down: 
   (mem1: HS.mem) -> 
