vale/specs/interop/Interop.Assumptions.fst
@@ -4,22 +4,41 @@ module ST = FStar.HyperStack.ST
 module HS = FStar.HyperStack
 module MS = X64.Machine_s
 
-assume 
-val st_put (#a:Type) (p:HS.mem -> Type0) (f:(h0:HS.mem{p h0}) -> GTot (x:(a & HS.mem){ST.equal_domains h0 (snd x)}))
-  : ST.Stack a 
+assume
+val st_put
+      (#a:Type)
+      (p:HS.mem -> Type0)
+      (f:(h0:HS.mem{p h0} ->
+           GTot (x:(a & HS.mem){ST.equal_domains h0 (snd x)})))
+  : ST.Stack a
     (requires p)
     (ensures fun h0 x h1 -> f h0 == (x,h1))
 
 //The map from buffers to addresses in the heap, that remains abstract
-assume 
+assume
 val addrs: addr_map
 
 //The initial registers and xmms
-assume 
+assume
 val init_regs: MS.reg -> MS.nat64
 
-assume 
+assume
 val init_xmms: MS.xmm -> MS.quad32
 
 // Abstract current operating system from Low*
-assume val win: bool
+assume
+val win: bool
+
+(* If two refs have the same address, and are in the heap, they are equal *)
+assume
+val ref_extensionality
+      (#a:Type0)
+      (#rel:Preorder.preorder a)
+      (h:Heap.heap)
+      (r1 r2:Heap.mref a rel)
+  : Lemma
+     (ensures Heap.contains h r1 /\
+              Heap.contains h r2 /\
+              Heap.addr_of r1 = Heap.addr_of r2 ==>
+              r1 == r2)
+
