vale/specs/interop/Interop.Base.fst
@@ -4,12 +4,12 @@ module B = LowStar.Buffer
 module BS = X64.Bytes_Semantics_s
 module BV = LowStar.BufferView
 module HS = FStar.HyperStack
-module LU = LowStar.Util
 module ME = X64.Memory
 module TS = X64.Taint_Semantics_s
 module MS = X64.Machine_s
-let reduce = ()
+let __reduce__ = ()
 
+[@__reduce__]
 let view_n (x:ME.typ) =
   let open ME in
   match x with
@@ -21,6 +21,7 @@ let view_n (x:ME.typ) =
 
 let b8 = B.buffer UInt8.t
 
+[@__reduce__]
 let lowstar_buffer (t:ME.typ) = b:b8{B.length b % view_n t == 0}
 
 //TODO: This should be provided by X64.Memory
@@ -28,16 +29,16 @@ let buffer_equiv (t:ME.typ)
   : Lemma (ME.buffer t == lowstar_buffer t)
   = admit()
 
-[@reduce]
+[@__reduce__]
 let coerce (x:'a{'a == 'b}) : 'b = x
 
-[@reduce]
+[@__reduce__]
 let as_lowstar_buffer (#t:ME.typ) (x:ME.buffer t)
   : Tot (lowstar_buffer t)
   = buffer_equiv t;
     coerce x
 
-[@reduce]
+[@__reduce__]
 let as_vale_buffer (#t:ME.typ) (x:lowstar_buffer t)
   : Tot (b:ME.buffer t)
   = buffer_equiv t;
@@ -55,7 +56,7 @@ let normal (#a:Type) (x:a) : a =
   FStar.Pervasives.norm
     [iota;
      zeta;
-     delta_attr [`%reduce];
+     delta_attr [`%__reduce__; `%BigOps.__reduce__];
      delta_only [`%TD_Buffer?;
                  `%BS.Mkstate?.ok;
                  `%BS.Mkstate?.regs;
@@ -66,7 +67,9 @@ let normal (#a:Type) (x:a) : a =
                  `%TS.MktraceState?.trace;
                  `%TS.MktraceState?.memTaint;
                  `%FStar.FunctionalExtensionality.on_dom;
-                 `%FStar.FunctionalExtensionality.on// ;
+                 `%FStar.FunctionalExtensionality.on;
+                 `%List.Tot.fold_right_gtot;
+                 `%List.Tot.map_gtot;
                  // `%Interop.list_disjoint_or_eq;
                  // `%Interop.list_live
                  ];
@@ -77,7 +80,7 @@ let normal (#a:Type) (x:a) : a =
 ////////////////////////////////////////////////////////////////////////////////
 
 #set-options "--initial_ifuel 1"
-[@reduce]
+[@__reduce__]
 let base_typ_as_type : X64.Memory.base_typ -> Type =
   let open ME in
   function
@@ -87,7 +90,7 @@ let base_typ_as_type : X64.Memory.base_typ -> Type =
   | TUInt64 -> UInt64.t
   | TUInt128 -> UInt128.t
 
-[@reduce]
+[@__reduce__]
 let td_as_type : td -> Type =
   let open ME in
   function
@@ -101,35 +104,35 @@ let arg = t:td & td_as_type t
 // n_arrow: Arrows with a generic number of vale types as the domain
 //          and a result type `codom` that does not depend on the domain
 ////////////////////////////////////////////////////////////////////////////////
-[@(unifier_hint_injective) (reduce)]
+[@(unifier_hint_injective) (__reduce__)]
 let rec n_arrow (dom:list td) (codom:Type) =
   match dom with
   | [] -> codom
   | hd::tl -> td_as_type hd -> n_arrow tl codom
 
-[@(unifier_hint_injective) (reduce)]
+[@(unifier_hint_injective) (__reduce__)]
 let arr (dom:Type) (codom:Type) = dom -> codom
 
-[@reduce]
+[@__reduce__]
 let elim_1 (#dom:list td{Cons? dom})
            (#r:Type)
            (f:n_arrow dom r)
     : td_as_type (Cons?.hd dom) -> n_arrow (Cons?.tl dom) r =
     f
 
-[@reduce]
+[@__reduce__]
 let elim_nil (#dom:list td{Nil? dom})
            (#r:Type)
            (f:n_arrow dom r)
     : r =
     f
 
-[@reduce]
+[@__reduce__]
 let intro_n_arrow_nil (a:Type) (x:a)
   : n_arrow [] a
   = x
 
-[@reduce]
+[@__reduce__]
 let intro_n_arrow_cons (hd:td) (b:Type) (tl:list td)
                        (x:td_as_type hd -> n_arrow tl b)
   : n_arrow (hd::tl) b
@@ -139,26 +142,26 @@ let intro_n_arrow_cons (hd:td) (b:Type) (tl:list td)
 // n_dep_arrow: Arrows with a generic number of vale types as the domain
 //              and a result type codom that depends on the domain
 ////////////////////////////////////////////////////////////////////////////////
-[@(unifier_hint_injective) (reduce)]
+[@(unifier_hint_injective) (__reduce__)]
 let rec n_dep_arrow (dom:list td) (codom: n_arrow dom Type) =
   match dom with
   | [] -> codom
   | hd::tl -> x:td_as_type hd -> n_dep_arrow tl (elim_1 codom x)
 
-[@reduce]
+[@__reduce__]
 let intro_dep_arrow_nil (b:Type)
                         (f:b)
   : n_dep_arrow [] b
   = f
 
-[@reduce]
+[@__reduce__]
 let intro_dep_arrow_1 (a:td)
                       (b:n_arrow [a] Type)
                       (f:(x:td_as_type a -> elim_1 b x))
   : n_dep_arrow [a] b
   = f
 
-[@reduce]
+[@__reduce__]
 let intro_dep_arrow_cons (hd:td)
                          (tl:list td)
                          (b: n_arrow (hd::tl) Type)
@@ -166,13 +169,13 @@ let intro_dep_arrow_cons (hd:td)
   : n_dep_arrow (hd::tl) b
   = f
 
-[@reduce]
+[@__reduce__]
 let elim_dep_arrow_nil (#codom:n_arrow [] Type)
                        (f:n_dep_arrow [] codom)
     : elim_nil codom
    = f
 
-[@reduce]
+[@__reduce__]
 let elim_dep_arrow_cons (hd:td)
                         (tl:list td)
                         (#codom:n_arrow (hd::tl) Type)
@@ -199,45 +202,45 @@ type addr_map = m:(b8 -> ME.nat64){
 
 ////////////////////////////////////////////////////////////////////////////////
 
-[@reduce]
+[@__reduce__]
 let disjoint_or_eq_1 (a:arg) (b:arg) =
     match a, b with
     | (| TD_Buffer tx, xb |), (| TD_Buffer ty, yb |) ->
       B.disjoint #UInt8.t xb yb \/ eq2 #b8 xb yb
     | _ -> True
 
-[@reduce]
+[@__reduce__]
 let disjoint_or_eq (l:list arg) =
   BigOps.pairwise_and disjoint_or_eq_1  l
 
-[@reduce]
+[@__reduce__]
 let live_arg (h:HS.mem) (x:arg) =
     match x with
     | (|TD_Buffer _, x|) -> B.live h x
     | _ -> True
 
-[@reduce]
+[@__reduce__]
 let all_live (h:HS.mem) (bs:list arg) =
   BigOps.big_and (live_arg h) bs
 
-[@reduce]
+[@__reduce__]
 let mem_roots_p (h0:HS.mem) (args:list arg) =
   disjoint_or_eq args /\
   all_live h0 args
 
-[@reduce]
+[@__reduce__]
 let mem_roots (args:list arg) =
     h0:HS.mem{ mem_roots_p h0 args }
 
-[@reduce]
+[@__reduce__]
 let arg_loc (x:arg) : GTot B.loc =
     match x with
     | (|TD_Buffer _, x|) -> B.loc_buffer x
     | _ -> B.loc_none
 
-[@reduce]
+[@__reduce__]
 let loc_args (args:list arg) : GTot B.loc =
-    LowStar.Util.loc_union_l (BigOps.map_gtot arg_loc args)
+    B.loc_union_l (List.Tot.map_gtot arg_loc args)
 
 let all_live_cons (hd:arg) (tl:list arg) (h0:HS.mem)
   : Lemma 
@@ -250,7 +253,8 @@ let disjoint_or_eq_def (l:list arg)
 
 let disjoint_or_eq_cons (hd:arg) (tl:list arg)
   : Lemma (disjoint_or_eq (hd::tl) <==> (BigOps.big_and (disjoint_or_eq_1 hd) tl /\ disjoint_or_eq tl))
-  = BigOps.pairwise_and_cons disjoint_or_eq_1 hd tl;
+  = BigOps.pairwise_and'_cons disjoint_or_eq_1 hd tl;
+    BigOps.normal_eq (BigOps.big_and' (disjoint_or_eq_1 hd) tl);
     disjoint_or_eq_def (hd::tl)
 
 let rec mem_roots_p_modifies_none (args:list arg) (h0:HS.mem) (h1:HS.mem)
@@ -266,6 +270,7 @@ let rec mem_roots_p_modifies_none (args:list arg) (h0:HS.mem) (h1:HS.mem)
       disjoint_or_eq_cons hd tl;
       mem_roots_p_modifies_none tl h0 h1
 
+[@__reduce__]
 let arg_of_lb #t (x:lowstar_buffer (ME.TBase t)) : arg = (| TD_Buffer t, x |)
 
 let rec disjoint_or_eq_fresh
